Update to Isabelle2024 (#14)
Co-authored-by: Conrad <cnrdwtt@gmail.com>
Co-authored-by: MajaTr <50637110+MajaTr@users.noreply.github.com>
Co-authored-by: Peter Lammich <plammich@gmail.com>
Co-authored-by: Maja Trela <maja.ada0@gmail.com>
Co-authored-by: lammich <lammich@in.tum.de>

WebAssembly/Wasm.thy
@@ -4,37 +4,46 @@ theory Wasm imports Wasm_Base_Defs begin
 inductive b_e_typing :: "[t_context, b_e list, tf] \<Rightarrow> bool" ("_ \<turnstile> _ : _" 60) where
   \<comment> \<open>\<open>num ops\<close>\<close>
   const:"\<C> \<turnstile> [C v] :([] _> [(typeof v)])"
-| unop:"unop_t_agree op t   \<Longrightarrow> \<C> \<turnstile> [Unop t op]  : ([t]   _> [t])"
-| binop:"binop_t_agree op t \<Longrightarrow> \<C> \<turnstile> [Binop t op] : ([t,t] _> [t])"
-| testop:"is_int_t t   \<Longrightarrow> \<C> \<turnstile> [Testop t _]      : ([t]   _> [T_i32])"
-| relop:"relop_t_agree op t   \<Longrightarrow> \<C> \<turnstile> [Relop t op] : ([t,t] _> [T_i32])"
+| unop:"unop_t_num_agree op t   \<Longrightarrow> \<C> \<turnstile> [Unop t op]  : ([T_num t]   _> [T_num t])"
+| binop:"binop_t_num_agree op t \<Longrightarrow> \<C> \<turnstile> [Binop t op] : ([T_num t,T_num t] _> [T_num t])"
+| testop:"is_int_t_num t   \<Longrightarrow> \<C> \<turnstile> [Testop t _]      : ([T_num t]   _> [T_num T_i32])"
+| relop:"relop_t_num_agree op t   \<Longrightarrow> \<C> \<turnstile> [Relop t op] : ([T_num t,T_num t] _> [T_num T_i32])"
+  \<comment> \<open>\<open>vector ops\<close>\<close>
+| unop_vec:"\<C> \<turnstile> [Unop_vec op]  : ([T_vec T_v128]   _> [T_vec T_v128])"
+| binop_vec:"\<lbrakk>binop_vec_wf op\<rbrakk> \<Longrightarrow> \<C> \<turnstile> [Binop_vec op]  : ([T_vec T_v128, T_vec T_v128]   _> [T_vec T_v128])"
+| ternop_vec:"\<C> \<turnstile> [Ternop_vec op]  : ([T_vec T_v128, T_vec T_v128, T_vec T_v128]   _> [T_vec T_v128])"
+| test_vec:"\<C> \<turnstile> [Test_vec op]  : ([T_vec T_v128]   _> [T_num T_i32])"
+| shift_vec:"\<C> \<turnstile> [Shift_vec op]  : ([T_vec T_v128, T_num T_i32]   _> [T_vec T_v128])"
+| splat_vec:"\<C> \<turnstile> [Splat_vec sv]  : ([T_num (vec_lane_t sv)]   _> [T_vec T_v128])"
+| extract_vec:"\<lbrakk>i < vec_num sv; sx = U \<or> vec_length sv \<le> 2\<rbrakk> \<Longrightarrow> \<C> \<turnstile> [Extract_vec sv sx i]  : ([T_vec T_v128]   _> [T_num (vec_lane_t sv)])"
+| replace_vec:"i < vec_num sv \<Longrightarrow> \<C> \<turnstile> [Replace_vec sv i]  : ([T_vec T_v128, T_num (vec_lane_t sv)]   _> [T_vec T_v128])"
   \<comment> \<open>\<open>convert\<close>\<close>
-| convert:"\<lbrakk>(t1 \<noteq> t2); (sx = None) = ((is_float_t t1 \<and> is_float_t t2) \<or> (is_int_t t1 \<and> is_int_t t2 \<and> (t_length t1 < t_length t2)))\<rbrakk> \<Longrightarrow> \<C> \<turnstile> [Cvtop t1 Convert t2 sx] : ([t2] _> [t1])"
+| convert:"\<lbrakk>(t1 \<noteq> t2); (sat_sx = None) = ((is_float_t_num t1 \<and> is_float_t_num t2) \<or> (is_int_t_num t1 \<and> is_int_t_num t2 \<and> (t_num_length t1 < t_num_length t2)))\<rbrakk> \<Longrightarrow> \<C> \<turnstile> [Cvtop t1 Convert t2 sat_sx] : ([T_num t2] _> [T_num t1])"
   \<comment> \<open>\<open>reinterpret\<close>\<close>
-| reinterpret:"\<lbrakk>(t1 \<noteq> t2); t_length t1 = t_length t2\<rbrakk> \<Longrightarrow> \<C> \<turnstile> [Cvtop t1 Reinterpret t2 None] : ([t2] _> [t1])"
+| reinterpret:"\<lbrakk>(t1 \<noteq> t2); t_num_length t1 = t_num_length t2\<rbrakk> \<Longrightarrow> \<C> \<turnstile> [Cvtop t1 Reinterpret t2 None] : ([T_num t2] _> [T_num t1])"
   \<comment> \<open>\<open>unreachable, nop, drop, select\<close>\<close>
 | unreachable:"\<C> \<turnstile> [Unreachable] : (ts _> ts')"
 | nop:"\<C> \<turnstile> [Nop] : ([] _> [])"
 | drop:"\<C> \<turnstile> [Drop] : ([t] _> [])"
-| select:"\<C> \<turnstile> [Select] : ([t,t,T_i32] _> [t])"
+| select:"\<C> \<turnstile> [Select] : ([t,t,T_num T_i32] _> [t])"
   \<comment> \<open>\<open>block\<close>\<close>
-| block:"\<lbrakk>tf = (tn _> tm); \<C>\<lparr>label := ([tm] @ (label \<C>))\<rparr> \<turnstile> es : (tn _> tm)\<rbrakk> \<Longrightarrow> \<C> \<turnstile> [Block tf es] : (tn _> tm)"
+| block:"\<lbrakk>tb_tf_t \<C> tb = Some (tn _> tm); \<C>\<lparr>label := ([tm] @ (label \<C>))\<rparr> \<turnstile> es : (tn _> tm)\<rbrakk> \<Longrightarrow> \<C> \<turnstile> [Block tb es] : (tn _> tm)"
   \<comment> \<open>\<open>loop\<close>\<close>
-| loop:"\<lbrakk>tf = (tn _> tm); \<C>\<lparr>label := ([tn] @ (label \<C>))\<rparr> \<turnstile> es : (tn _> tm)\<rbrakk> \<Longrightarrow> \<C> \<turnstile> [Loop tf es] : (tn _> tm)"
+| loop:"\<lbrakk>tb_tf_t \<C> tb = Some (tn _> tm); \<C>\<lparr>label := ([tn] @ (label \<C>))\<rparr> \<turnstile> es : (tn _> tm)\<rbrakk> \<Longrightarrow> \<C> \<turnstile> [Loop tb es] : (tn _> tm)"
   \<comment> \<open>\<open>if then else\<close>\<close>
-| if_wasm:"\<lbrakk>tf = (tn _> tm); \<C>\<lparr>label := ([tm] @ (label \<C>))\<rparr> \<turnstile> es1 : (tn _> tm); \<C>\<lparr>label := ([tm] @ (label \<C>))\<rparr> \<turnstile> es2 : (tn _> tm)\<rbrakk> \<Longrightarrow> \<C> \<turnstile> [If tf es1 es2] : (tn @ [T_i32] _> tm)"
+| if_wasm:"\<lbrakk>tb_tf_t \<C> tb = Some (tn _> tm); \<C>\<lparr>label := ([tm] @ (label \<C>))\<rparr> \<turnstile> es1 : (tn _> tm); \<C>\<lparr>label := ([tm] @ (label \<C>))\<rparr> \<turnstile> es2 : (tn _> tm)\<rbrakk> \<Longrightarrow> \<C> \<turnstile> [If tb es1 es2] : (tn @ [T_num T_i32] _> tm)"
   \<comment> \<open>\<open>br\<close>\<close>
 | br:"\<lbrakk>i < length(label \<C>); (label \<C>)!i = ts\<rbrakk> \<Longrightarrow> \<C> \<turnstile> [Br i] : (t1s @ ts _> t2s)"
   \<comment> \<open>\<open>br_if\<close>\<close>
-| br_if:"\<lbrakk>i < length(label \<C>); (label \<C>)!i = ts\<rbrakk> \<Longrightarrow> \<C> \<turnstile> [Br_if i] : (ts @ [T_i32] _> ts)"
+| br_if:"\<lbrakk>i < length(label \<C>); (label \<C>)!i = ts\<rbrakk> \<Longrightarrow> \<C> \<turnstile> [Br_if i] : (ts @ [T_num T_i32] _> ts)"
   \<comment> \<open>\<open>br_table\<close>\<close>
-| br_table:"\<lbrakk>list_all (\<lambda>i. i < length(label \<C>) \<and> (label \<C>)!i = ts) (is@[i])\<rbrakk> \<Longrightarrow> \<C> \<turnstile> [Br_table is i] : (t1s @ ts @ [T_i32] _> t2s)"
+| br_table:"\<lbrakk>list_all (\<lambda>i. i < length(label \<C>) \<and> (label \<C>)!i = ts) (is@[i])\<rbrakk> \<Longrightarrow> \<C> \<turnstile> [Br_table is i] : (t1s @ ts @ [T_num T_i32] _> t2s)"
   \<comment> \<open>\<open>return\<close>\<close>
 | return:"\<lbrakk>(return \<C>) = Some ts\<rbrakk> \<Longrightarrow> \<C> \<turnstile> [Return] : (t1s @ ts _> t2s)"
   \<comment> \<open>\<open>call\<close>\<close>
 | call:"\<lbrakk>i < length(func_t \<C>); (func_t \<C>)!i = tf\<rbrakk> \<Longrightarrow> \<C> \<turnstile> [Call i] : tf"
   \<comment> \<open>\<open>call_indirect\<close>\<close>
-| call_indirect:"\<lbrakk>i < length(types_t \<C>); (types_t \<C>)!i = (t1s _> t2s); length (table \<C>) \<ge> 1\<rbrakk> \<Longrightarrow> \<C> \<turnstile> [Call_indirect i] : (t1s @ [T_i32] _> t2s)"
+| call_indirect:"\<lbrakk>i < length(types_t \<C>); (types_t \<C>)!i = (t1s _> t2s); length (table \<C>) \<ge> 1\<rbrakk> \<Longrightarrow> \<C> \<turnstile> [Call_indirect i] : (t1s @ [T_num T_i32] _> t2s)"
   \<comment> \<open>\<open>get_local\<close>\<close>
 | get_local:"\<lbrakk>i < length(local \<C>); (local \<C>)!i = t\<rbrakk> \<Longrightarrow> \<C> \<turnstile> [Get_local i] : ([] _> [t])"
   \<comment> \<open>\<open>set_local\<close>\<close>
@@ -46,13 +55,19 @@ inductive b_e_typing :: "[t_context, b_e list, tf] \<Rightarrow> bool" ("_ \<tur
   \<comment> \<open>\<open>set_global\<close>\<close>
 | set_global:"\<lbrakk>i < length(global \<C>); tg_t ((global \<C>)!i) = t; is_mut ((global \<C>)!i)\<rbrakk> \<Longrightarrow> \<C> \<turnstile> [Set_global i] : ([t] _> [])"
   \<comment> \<open>\<open>load\<close>\<close>
-| load:"\<lbrakk>length (memory \<C>) \<ge> 1; load_store_t_bounds a (option_projl tp_sx) t\<rbrakk> \<Longrightarrow> \<C> \<turnstile> [Load t tp_sx a off] : ([T_i32] _> [t])"
+| load:"\<lbrakk>length (memory \<C>) \<ge> 1; load_store_t_bounds a (option_projl tp_sx) t\<rbrakk> \<Longrightarrow> \<C> \<turnstile> [Load t tp_sx a off] : ([T_num T_i32] _> [T_num t])"
   \<comment> \<open>\<open>store\<close>\<close>
-| store:"\<lbrakk>length (memory \<C>) \<ge> 1; load_store_t_bounds a tp t\<rbrakk> \<Longrightarrow> \<C> \<turnstile> [Store t tp a off] : ([T_i32,t] _> [])"
+| store:"\<lbrakk>length (memory \<C>) \<ge> 1; load_store_t_bounds a tp t\<rbrakk> \<Longrightarrow> \<C> \<turnstile> [Store t tp a off] : ([T_num T_i32,T_num t] _> [])"
+  \<comment> \<open>\<open>load_vec\<close>\<close>
+| load_vec:"\<lbrakk>length (memory \<C>) \<ge> 1; load_vec_t_bounds lvop a\<rbrakk> \<Longrightarrow> \<C> \<turnstile> [Load_vec lvop a off] : ([T_num T_i32] _> [T_vec T_v128])"
+  \<comment> \<open>\<open>load_lane_vec\<close>\<close>
+| load_lane_vec:"\<lbrakk>length (memory \<C>) \<ge> 1; i < vec_i_num svi \<and> 2^a \<le> (vec_i_length svi)\<rbrakk> \<Longrightarrow> \<C> \<turnstile> [Load_lane_vec svi i a off] : ([T_num T_i32, T_vec T_v128] _> [T_vec T_v128])"
+  \<comment> \<open>\<open>store_vec\<close>\<close>
+| store_vec:"\<lbrakk>length (memory \<C>) \<ge> 1; store_vec_t_bounds svop a\<rbrakk> \<Longrightarrow> \<C> \<turnstile> [Store_vec svop a off] : ([T_num T_i32,T_vec T_v128] _> [])"
   \<comment> \<open>\<open>current_memory\<close>\<close>
-| current_memory:"length (memory \<C>) \<ge> 1 \<Longrightarrow> \<C> \<turnstile> [Current_memory] : ([] _> [T_i32])"
+| current_memory:"length (memory \<C>) \<ge> 1 \<Longrightarrow> \<C> \<turnstile> [Current_memory] : ([] _> [T_num T_i32])"
   \<comment> \<open>\<open>Grow_memory\<close>\<close>
-| grow_memory:"length (memory \<C>) \<ge> 1 \<Longrightarrow> \<C> \<turnstile> [Grow_memory] : ([T_i32] _> [T_i32])"
+| grow_memory:"length (memory \<C>) \<ge> 1 \<Longrightarrow> \<C> \<turnstile> [Grow_memory] : ([T_num T_i32] _> [T_num T_i32])"
   \<comment> \<open>\<open>empty program\<close>\<close>
 | empty:"\<C> \<turnstile> [] : ([] _> [])"
   \<comment> \<open>\<open>composition\<close>\<close>
@@ -115,6 +130,10 @@ and       l_typing :: "[s, (t list) option, f, e list, t list] \<Rightarrow> boo
 | "\<lbrakk>i < length (funcs \<S>); cl_type ((funcs \<S>)!i) = tf\<rbrakk> \<Longrightarrow> \<S>\<bullet>\<C>  \<turnstile> [Invoke i] : tf"
   (* label *)
 | "\<lbrakk>\<S>\<bullet>\<C> \<turnstile> e0s : (ts _> t2s); \<S>\<bullet>\<C>\<lparr>label := ([ts] @ (label \<C>))\<rparr> \<turnstile> es : ([] _> t2s); length ts = n\<rbrakk> \<Longrightarrow> \<S>\<bullet>\<C> \<turnstile> [Label n e0s es] : ([] _> t2s)"
+  (* Init_mem (instantiation) *)
+| "\<lbrakk>length (memory \<C>) \<ge> 1\<rbrakk> \<Longrightarrow> \<S>\<bullet>\<C>  \<turnstile> [Init_mem n bs] : ([] _> [])"
+  (* Init_tab (instantiation) *)
+| "\<lbrakk>length (table \<C>) \<ge> 1; list_all (\<lambda>ti. ti < length (funcs \<S>)) tis\<rbrakk> \<Longrightarrow> \<S>\<bullet>\<C>  \<turnstile> [Init_tab n tis] : ([] _> [])"
 (* section: l_typing *)
 | "\<lbrakk>frame_typing \<S> f \<C>; \<S>\<bullet>\<C>\<lparr>return := rs\<rparr> \<turnstile> es : ([] _> ts)\<rbrakk> \<Longrightarrow> \<S>\<bullet>rs \<tturnstile> f;es : ts"
 
@@ -135,19 +154,36 @@ inductive config_typing :: "[s, f, e list, t list] \<Rightarrow> bool" ("\<turns
 
 inductive reduce_simple :: "[e list, e list] \<Rightarrow> bool" ("\<lparr>_\<rparr> \<leadsto> \<lparr>_\<rparr>" 60) where
   \<comment> \<open>\<open>unary ops\<close>\<close>
-  unop:"\<lparr>[$C v, $(Unop t op)]\<rparr> \<leadsto> \<lparr>[$C (app_unop op v)]\<rparr>"
+  unop:"\<lparr>[$C\<^sub>n v, $(Unop t op)]\<rparr> \<leadsto> \<lparr>[$C\<^sub>n (app_unop op v)]\<rparr>"
   \<comment> \<open>\<open>binary ops\<close>\<close>
-| binop_Some:"\<lbrakk>app_binop op v1 v2 = (Some v)\<rbrakk> \<Longrightarrow> \<lparr>[$C v1, $C v2, $(Binop t op)]\<rparr> \<leadsto> \<lparr>[$C v]\<rparr>"
-| binop_None:"\<lbrakk>app_binop op v1 v2 = None\<rbrakk> \<Longrightarrow> \<lparr>[$C v1, $C v2, $(Binop t op)]\<rparr> \<leadsto> \<lparr>[Trap]\<rparr>"
+| binop_Some:"\<lbrakk>app_binop op v1 v2 = (Some v)\<rbrakk> \<Longrightarrow> \<lparr>[$C\<^sub>n v1, $C\<^sub>n v2, $(Binop t op)]\<rparr> \<leadsto> \<lparr>[$C\<^sub>n v]\<rparr>"
+| binop_None:"\<lbrakk>app_binop op v1 v2 = None\<rbrakk> \<Longrightarrow> \<lparr>[$C\<^sub>n v1, $C\<^sub>n v2, $(Binop t op)]\<rparr> \<leadsto> \<lparr>[Trap]\<rparr>"
   \<comment> \<open>\<open>testops\<close>\<close>
-| testop:"\<lparr>[$C v, $(Testop t op)]\<rparr> \<leadsto> \<lparr>[$C (app_testop op v)]\<rparr>"
+| testop:"\<lparr>[$C\<^sub>n v, $(Testop t op)]\<rparr> \<leadsto> \<lparr>[$C\<^sub>n (app_testop op v)]\<rparr>"
   \<comment> \<open>\<open>relops\<close>\<close>
-| relop:"\<lparr>[$C v1, $C v2, $(Relop t op)]\<rparr> \<leadsto> \<lparr>[$C (app_relop op v1 v2)]\<rparr>"
+| relop:"\<lparr>[$C\<^sub>n v1, $C\<^sub>n v2, $(Relop t op)]\<rparr> \<leadsto> \<lparr>[$C\<^sub>n (app_relop op v1 v2)]\<rparr>"
   \<comment> \<open>\<open>convert\<close>\<close>
-| convert_Some:"\<lbrakk>types_agree t1 v; cvt t2 sx v = (Some v')\<rbrakk> \<Longrightarrow> \<lparr>[$(C v), $(Cvtop t2 Convert t1 sx)]\<rparr> \<leadsto> \<lparr>[$(C v')]\<rparr>"
-| convert_None:"\<lbrakk>types_agree t1 v; cvt t2 sx v = None\<rbrakk> \<Longrightarrow> \<lparr>[$(C v), $(Cvtop t2 Convert t1 sx)]\<rparr> \<leadsto> \<lparr>[Trap]\<rparr>"
+| convert_Some:"\<lbrakk>(typeof_num v) = t1; cvt t2 sat_sx v = (Some v')\<rbrakk> \<Longrightarrow> \<lparr>[$(C\<^sub>n v), $(Cvtop t2 Convert t1 sat_sx)]\<rparr> \<leadsto> \<lparr>[$(C\<^sub>n v')]\<rparr>"
+| convert_None:"\<lbrakk>(typeof_num v) = t1; cvt t2 sat_sx v = None\<rbrakk> \<Longrightarrow> \<lparr>[$(C\<^sub>n v), $(Cvtop t2 Convert t1 sat_sx)]\<rparr> \<leadsto> \<lparr>[Trap]\<rparr>"
   \<comment> \<open>\<open>reinterpret\<close>\<close>
-| reinterpret:"types_agree t1 v \<Longrightarrow> \<lparr>[$(C v), $(Cvtop t2 Reinterpret t1 None)]\<rparr> \<leadsto> \<lparr>[$(C (wasm_deserialise (bits v) t2))]\<rparr>"
+| reinterpret:"(typeof_num v) = t1 \<Longrightarrow> \<lparr>[$(C\<^sub>n v), $(Cvtop t2 Reinterpret t1 None)]\<rparr> \<leadsto> \<lparr>[$(C\<^sub>n (wasm_reinterpret t2 v))]\<rparr>"
+  \<comment> \<open>\<open>unary vector ops\<close>\<close>
+| unop_vec:"\<lparr>[$C\<^sub>v v, $(Unop_vec op)]\<rparr> \<leadsto> \<lparr>[$C\<^sub>v (app_unop_vec op v)]\<rparr>"
+  \<comment> \<open>\<open>binary vector ops\<close>\<close>
+| binop_vec_Some:"\<lbrakk>app_binop_vec op v1 v2 = Some v\<rbrakk> \<Longrightarrow> \<lparr>[$C\<^sub>v v1, $C\<^sub>v v2, $(Binop_vec op)]\<rparr> \<leadsto> \<lparr>[$C\<^sub>v v]\<rparr>"
+| binop_vec_None:"\<lbrakk>app_binop_vec op v1 v2 = None\<rbrakk> \<Longrightarrow> \<lparr>[$C\<^sub>v v1, $C\<^sub>v v2, $(Binop_vec op)]\<rparr> \<leadsto> \<lparr>[Trap]\<rparr>"
+  \<comment> \<open>\<open>ternary vector ops\<close>\<close>
+| ternop_vec:"\<lparr>[$C\<^sub>v v1, $C\<^sub>v v2, $C\<^sub>v v3, $(Ternop_vec op)]\<rparr> \<leadsto> \<lparr>[$C\<^sub>v (app_ternop_vec op v1 v2 v3)]\<rparr>"
+  \<comment> \<open>\<open>test vector ops\<close>\<close>
+| test_vec:"\<lparr>[$C\<^sub>v v, $(Test_vec op)]\<rparr> \<leadsto> \<lparr>[$C\<^sub>n (ConstInt32 (app_test_vec op v))]\<rparr>"
+  \<comment> \<open>\<open>shift vector ops\<close>\<close>
+| shift_vec:"\<lparr>[$C\<^sub>v v, $C\<^sub>n (ConstInt32 n), $(Shift_vec op)]\<rparr> \<leadsto> \<lparr>[$C\<^sub>v (app_shift_vec op v n)]\<rparr>"
+  \<comment> \<open>\<open>splat vector ops\<close>\<close>
+| splat_vec:"\<lparr>[$C\<^sub>n v, $(Splat_vec sv)]\<rparr> \<leadsto> \<lparr>[$C\<^sub>v (app_splat_vec sv v)]\<rparr>"
+  \<comment> \<open>\<open>extract vector ops\<close>\<close>
+| extract_vec:"\<lparr>[$C\<^sub>v v, $(Extract_vec sv sx i)]\<rparr> \<leadsto> \<lparr>[$C\<^sub>n (app_extract_vec sv sx i v)]\<rparr>"
+  \<comment> \<open>\<open>replace vector ops\<close>\<close>
+| replace_vec:"\<lparr>[$C\<^sub>v v, $C\<^sub>n vn, $(Replace_vec sv i)]\<rparr> \<leadsto> \<lparr>[$C\<^sub>v (app_replace_vec sv i v vn)]\<rparr>"
   \<comment> \<open>\<open>unreachable\<close>\<close>
 | unreachable:"\<lparr>[$ Unreachable]\<rparr> \<leadsto> \<lparr>[Trap]\<rparr>"
   \<comment> \<open>\<open>nop\<close>\<close>
@@ -155,26 +191,22 @@ inductive reduce_simple :: "[e list, e list] \<Rightarrow> bool" ("\<lparr>_\<rp
   \<comment> \<open>\<open>drop\<close>\<close>
 | drop:"\<lparr>[$(C v), ($ Drop)]\<rparr> \<leadsto> \<lparr>[]\<rparr>"
   \<comment> \<open>\<open>select\<close>\<close>
-| select_false:"int_eq n 0 \<Longrightarrow> \<lparr>[$(C v1), $(C v2), $C (ConstInt32 n), ($ Select)]\<rparr> \<leadsto> \<lparr>[$(C v2)]\<rparr>"
-| select_true:"int_ne n 0 \<Longrightarrow> \<lparr>[$(C v1), $(C v2), $C (ConstInt32 n), ($ Select)]\<rparr> \<leadsto> \<lparr>[$(C v1)]\<rparr>"
-  \<comment> \<open>\<open>block\<close>\<close>
-| block:"\<lbrakk>length vs = n; length t1s = n; length t2s = m\<rbrakk> \<Longrightarrow> \<lparr>($C* vs) @ [$(Block (t1s _> t2s) es)]\<rparr> \<leadsto> \<lparr>[Label m [] (($C* vs) @ ($* es))]\<rparr>"
-  \<comment> \<open>\<open>loop\<close>\<close>
-| loop:"\<lbrakk>length vs = n; length t1s = n; length t2s = m\<rbrakk> \<Longrightarrow> \<lparr>($C* vs) @ [$(Loop (t1s _> t2s) es)]\<rparr> \<leadsto> \<lparr>[Label n [$(Loop (t1s _> t2s) es)] (($C* vs) @ ($* es))]\<rparr>"
+| select_false:"int_eq n 0 \<Longrightarrow> \<lparr>[$(C v1), $(C v2), $C\<^sub>n (ConstInt32 n), ($ Select)]\<rparr> \<leadsto> \<lparr>[$(C v2)]\<rparr>"
+| select_true:"int_ne n 0 \<Longrightarrow> \<lparr>[$(C v1), $(C v2), $C\<^sub>n (ConstInt32 n), ($ Select)]\<rparr> \<leadsto> \<lparr>[$(C v1)]\<rparr>"
   \<comment> \<open>\<open>if\<close>\<close>
-| if_false:"int_eq n 0 \<Longrightarrow> \<lparr>[$C (ConstInt32 n), $(If tf e1s e2s)]\<rparr> \<leadsto> \<lparr>[$(Block tf e2s)]\<rparr>"
-| if_true:"int_ne n 0 \<Longrightarrow> \<lparr>[$C (ConstInt32 n), $(If tf e1s e2s)]\<rparr> \<leadsto> \<lparr>[$(Block tf e1s)]\<rparr>"
+| if_false:"int_eq n 0 \<Longrightarrow> \<lparr>[$C\<^sub>n (ConstInt32 n), $(If tb e1s e2s)]\<rparr> \<leadsto> \<lparr>[$(Block tb e2s)]\<rparr>"
+| if_true:"int_ne n 0 \<Longrightarrow> \<lparr>[$C\<^sub>n (ConstInt32 n), $(If tb e1s e2s)]\<rparr> \<leadsto> \<lparr>[$(Block tb e1s)]\<rparr>"
   \<comment> \<open>\<open>label\<close>\<close>
 | label_const:"\<lparr>[Label n es ($C* vs)]\<rparr> \<leadsto> \<lparr>($C* vs)\<rparr>"
 | label_trap:"\<lparr>[Label n es [Trap]]\<rparr> \<leadsto> \<lparr>[Trap]\<rparr>"
   \<comment> \<open>\<open>br\<close>\<close>
 | br:"\<lbrakk>length vs = n; Lfilled i lholed (($C* vs) @ [$(Br i)]) LI\<rbrakk> \<Longrightarrow> \<lparr>[Label n es LI]\<rparr> \<leadsto> \<lparr>($C* vs) @ es\<rparr>"
   \<comment> \<open>\<open>br_if\<close>\<close>
-| br_if_false:"int_eq n 0 \<Longrightarrow> \<lparr>[$C (ConstInt32 n), $(Br_if i)]\<rparr> \<leadsto> \<lparr>[]\<rparr>"
-| br_if_true:"int_ne n 0 \<Longrightarrow> \<lparr>[$C (ConstInt32 n), $(Br_if i)]\<rparr> \<leadsto> \<lparr>[$(Br i)]\<rparr>"
+| br_if_false:"int_eq n 0 \<Longrightarrow> \<lparr>[$C\<^sub>n (ConstInt32 n), $(Br_if i)]\<rparr> \<leadsto> \<lparr>[]\<rparr>"
+| br_if_true:"int_ne n 0 \<Longrightarrow> \<lparr>[$C\<^sub>n (ConstInt32 n), $(Br_if i)]\<rparr> \<leadsto> \<lparr>[$(Br i)]\<rparr>"
   \<comment> \<open>\<open>br_table\<close>\<close>
-| br_table:"\<lbrakk>length is > (nat_of_int c)\<rbrakk> \<Longrightarrow> \<lparr>[$C (ConstInt32 c), $(Br_table is i)]\<rparr> \<leadsto> \<lparr>[$(Br (is!(nat_of_int c)))]\<rparr>"
-| br_table_length:"\<lbrakk>length is \<le> (nat_of_int c)\<rbrakk> \<Longrightarrow> \<lparr>[$C (ConstInt32 c), $(Br_table is i)]\<rparr> \<leadsto> \<lparr>[$(Br i)]\<rparr>"
+| br_table:"\<lbrakk>length is > (nat_of_int c)\<rbrakk> \<Longrightarrow> \<lparr>[$C\<^sub>n (ConstInt32 c), $(Br_table is i)]\<rparr> \<leadsto> \<lparr>[$(Br (is!(nat_of_int c)))]\<rparr>"
+| br_table_length:"\<lbrakk>length is \<le> (nat_of_int c)\<rbrakk> \<Longrightarrow> \<lparr>[$C\<^sub>n (ConstInt32 c), $(Br_table is i)]\<rparr> \<leadsto> \<lparr>[$(Br i)]\<rparr>"
   \<comment> \<open>\<open>local\<close>\<close>
 | local_const:"\<lparr>[Frame n f ($C* vs)]\<rparr> \<leadsto> \<lparr>($C* vs)\<rparr>"
 | local_trap:"\<lparr>[Frame n f [Trap]]\<rparr> \<leadsto> \<lparr>[Trap]\<rparr>"
@@ -191,10 +223,10 @@ inductive reduce :: "[s, f, e list, s, f, e list] \<Rightarrow> bool" ("\<lparr>
   \<comment> \<open>\<open>call\<close>\<close>
 | call:"\<lparr>s;f;[$(Call j)]\<rparr> \<leadsto> \<lparr>s;f;[Invoke (sfunc_ind (f_inst f) j)]\<rparr>"
   \<comment> \<open>\<open>call_indirect\<close>\<close>
-| call_indirect_Some:"\<lbrakk>(f_inst f) = i; stab s i (nat_of_int c) = Some i_cl; stypes i j = tf; cl_type (funcs s!i_cl) = tf\<rbrakk> \<Longrightarrow> \<lparr>s;f;[$C (ConstInt32 c), $(Call_indirect j)]\<rparr> \<leadsto> \<lparr>s;f;[Invoke i_cl]\<rparr>"
-| call_indirect_None:"\<lbrakk>(f_inst f) = i; (stab s i (nat_of_int c) = Some i_cl \<and> stypes i j \<noteq> cl_type (funcs s!i_cl)) \<or> stab s i (nat_of_int c) = None\<rbrakk> \<Longrightarrow> \<lparr>s;f;[$C (ConstInt32 c), $(Call_indirect j)]\<rparr> \<leadsto> \<lparr>s;f;[Trap]\<rparr>"
+| call_indirect_Some:"\<lbrakk>(f_inst f) = i; stab s i (nat_of_int c) = Some i_cl; stypes i j = tf; cl_type (funcs s!i_cl) = tf\<rbrakk> \<Longrightarrow> \<lparr>s;f;[$C\<^sub>n (ConstInt32 c), $(Call_indirect j)]\<rparr> \<leadsto> \<lparr>s;f;[Invoke i_cl]\<rparr>"
+| call_indirect_None:"\<lbrakk>(f_inst f) = i; (stab s i (nat_of_int c) = Some i_cl \<and> stypes i j \<noteq> cl_type (funcs s!i_cl)) \<or> stab s i (nat_of_int c) = None\<rbrakk> \<Longrightarrow> \<lparr>s;f;[$C\<^sub>n (ConstInt32 c), $(Call_indirect j)]\<rparr> \<leadsto> \<lparr>s;f;[Trap]\<rparr>"
   \<comment> \<open>\<open>invoke\<close>\<close>
-| invoke_native:"\<lbrakk>(funcs s!i_cl) = Func_native j (t1s _> t2s) ts es; ves = ($C* vcs); length vcs = n; length ts = k; length t1s = n; length t2s = m; (n_zeros ts = zs) \<rbrakk> \<Longrightarrow> \<lparr>s;f;ves @ [Invoke i_cl]\<rparr> \<leadsto> \<lparr>s;f;[Frame m \<lparr> f_locs = vcs@zs, f_inst = j \<rparr> [$(Block ([] _> t2s) es)]]\<rparr>"
+| invoke_native:"\<lbrakk>(funcs s!i_cl) = Func_native j (t1s _> t2s) ts es; ves = ($C* vcs); length vcs = n; length ts = k; length t1s = n; length t2s = m; (n_zeros ts = zs) \<rbrakk> \<Longrightarrow> \<lparr>s;f;ves @ [Invoke i_cl]\<rparr> \<leadsto> \<lparr>s;f;[Frame m \<lparr> f_locs = vcs@zs, f_inst = j \<rparr> [(Label m [] ($*es))]]\<rparr>"
 | invoke_host_Some:"\<lbrakk>(funcs s!i_cl) = Func_host (t1s _> t2s) h; ves = ($C* vcs); length vcs = n; length t1s = n; length t2s = m; host_apply s (t1s _> t2s) h vcs hs (Some (s', vcs'))\<rbrakk> \<Longrightarrow> \<lparr>s;f;ves @ [Invoke i_cl]\<rparr> \<leadsto> \<lparr>s';f;($C* vcs')\<rparr>"
 | invoke_host_None:"\<lbrakk>(funcs s!i_cl) = Func_host (t1s _> t2s) h; ves = ($C* vcs); length vcs = n; length t1s = n; length t2s = m\<rbrakk> \<Longrightarrow> \<lparr>s;f;ves @ [Invoke i_cl]\<rparr> \<leadsto> \<lparr>s;f;[Trap]\<rparr>"
   \<comment> \<open>\<open>get_local\<close>\<close>
@@ -206,28 +238,46 @@ inductive reduce :: "[s, f, e list, s, f, e list] \<Rightarrow> bool" ("\<lparr>
   \<comment> \<open>\<open>set_global\<close>\<close>
 | set_global:"supdate_glob s (f_inst f) j v = s' \<Longrightarrow> \<lparr>s;f;[$(C v), $(Set_global j)]\<rparr> \<leadsto> \<lparr>s';f;[]\<rparr>"
   \<comment> \<open>\<open>load\<close>\<close>
-| load_Some:"\<lbrakk>smem_ind (f_inst f) = Some j; ((mems s)!j) = m; load m (nat_of_int k) off (t_length t) = Some bs\<rbrakk> \<Longrightarrow> \<lparr>s;f;[$C (ConstInt32 k), $(Load t None a off)]\<rparr> \<leadsto> \<lparr>s;f;[$C (wasm_deserialise bs t)]\<rparr>"
-| load_None:"\<lbrakk>smem_ind (f_inst f) = Some j; ((mems s)!j) = m; load m (nat_of_int k) off (t_length t) = None\<rbrakk> \<Longrightarrow> \<lparr>s;f;[$C (ConstInt32 k), $(Load t None a off)]\<rparr> \<leadsto> \<lparr>s;f;[Trap]\<rparr>"
+| load_Some:"\<lbrakk>smem_ind (f_inst f) = Some j; ((mems s)!j) = m; load m (nat_of_int k) off (t_num_length t) = Some bs\<rbrakk> \<Longrightarrow> \<lparr>s;f;[$C\<^sub>n (ConstInt32 k), $(Load t None a off)]\<rparr> \<leadsto> \<lparr>s;f;[$C\<^sub>n (wasm_deserialise_num bs t)]\<rparr>"
+| load_None:"\<lbrakk>smem_ind (f_inst f) = Some j; ((mems s)!j) = m; load m (nat_of_int k) off (t_num_length t) = None\<rbrakk> \<Longrightarrow> \<lparr>s;f;[$C\<^sub>n (ConstInt32 k), $(Load t None a off)]\<rparr> \<leadsto> \<lparr>s;f;[Trap]\<rparr>"
   \<comment> \<open>\<open>load packed\<close>\<close>
-| load_packed_Some:"\<lbrakk>smem_ind (f_inst f) = Some j; ((mems s)!j) = m; load_packed sx m (nat_of_int k) off (tp_length tp) (t_length t) = Some bs\<rbrakk> \<Longrightarrow> \<lparr>s;f;[$C (ConstInt32 k), $(Load t (Some (tp, sx)) a off)]\<rparr> \<leadsto> \<lparr>s;f;[$C (wasm_deserialise bs t)]\<rparr>"
-| load_packed_None:"\<lbrakk>smem_ind (f_inst f) = Some j; ((mems s)!j) = m; load_packed sx m (nat_of_int k) off (tp_length tp) (t_length t) = None\<rbrakk> \<Longrightarrow> \<lparr>s;f;[$C (ConstInt32 k), $(Load t (Some (tp, sx)) a off)]\<rparr> \<leadsto> \<lparr>s;f;[Trap]\<rparr>"
+| load_packed_Some:"\<lbrakk>smem_ind (f_inst f) = Some j; ((mems s)!j) = m; load_packed sx m (nat_of_int k) off (tp_num_length tp) (t_num_length t) = Some bs\<rbrakk> \<Longrightarrow> \<lparr>s;f;[$C\<^sub>n (ConstInt32 k), $(Load t (Some (tp, sx)) a off)]\<rparr> \<leadsto> \<lparr>s;f;[$C\<^sub>n (wasm_deserialise_num bs t)]\<rparr>"
+| load_packed_None:"\<lbrakk>smem_ind (f_inst f) = Some j; ((mems s)!j) = m; load_packed sx m (nat_of_int k) off (tp_num_length tp) (t_num_length t) = None\<rbrakk> \<Longrightarrow> \<lparr>s;f;[$C\<^sub>n (ConstInt32 k), $(Load t (Some (tp, sx)) a off)]\<rparr> \<leadsto> \<lparr>s;f;[Trap]\<rparr>"
   \<comment> \<open>\<open>store\<close>\<close>
-| store_Some:"\<lbrakk>types_agree t v; smem_ind (f_inst f) = Some j; ((mems s)!j) = m; store m (nat_of_int k) off (bits v) (t_length t) = Some mem'\<rbrakk> \<Longrightarrow> \<lparr>s;f;[$C (ConstInt32 k), $C v, $(Store t None a off)]\<rparr> \<leadsto> \<lparr>s\<lparr>mems:= ((mems s)[j := mem'])\<rparr>;f;[]\<rparr>"
-| store_None:"\<lbrakk>types_agree t v; smem_ind (f_inst f) = Some j; ((mems s)!j) = m; store m (nat_of_int k) off (bits v) (t_length t) = None\<rbrakk> \<Longrightarrow> \<lparr>s;f;[$C (ConstInt32 k), $C v, $(Store t None a off)]\<rparr> \<leadsto> \<lparr>s;f;[Trap]\<rparr>"
+| store_Some:"\<lbrakk>(typeof_num v) = t; smem_ind (f_inst f) = Some j; ((mems s)!j) = m; store m (nat_of_int k) off (bits_num v) (t_num_length t) = Some mem'\<rbrakk> \<Longrightarrow> \<lparr>s;f;[$C\<^sub>n (ConstInt32 k), $C\<^sub>n v, $(Store t None a off)]\<rparr> \<leadsto> \<lparr>s\<lparr>mems:= ((mems s)[j := mem'])\<rparr>;f;[]\<rparr>"
+| store_None:"\<lbrakk>(typeof_num v) = t; smem_ind (f_inst f) = Some j; ((mems s)!j) = m; store m (nat_of_int k) off (bits_num v) (t_num_length t) = None\<rbrakk> \<Longrightarrow> \<lparr>s;f;[$C\<^sub>n (ConstInt32 k), $C\<^sub>n v, $(Store t None a off)]\<rparr> \<leadsto> \<lparr>s;f;[Trap]\<rparr>"
   \<comment> \<open>\<open>store packed\<close>\<close> (* take only (tp_length tp) lower order bytes *)
-| store_packed_Some:"\<lbrakk>types_agree t v; smem_ind (f_inst f) = Some j; ((mems s)!j) = m; store_packed m (nat_of_int k) off (bits v) (tp_length tp) = Some mem'\<rbrakk> \<Longrightarrow> \<lparr>s;f;[$C (ConstInt32 k), $C v, $(Store t (Some tp) a off)]\<rparr> \<leadsto> \<lparr>s\<lparr>mems:= ((mems s)[j := mem'])\<rparr>;f;[]\<rparr>"
-| store_packed_None:"\<lbrakk>types_agree t v; smem_ind (f_inst f) = Some j; ((mems s)!j) = m; store_packed m (nat_of_int k) off (bits v) (tp_length tp) = None\<rbrakk> \<Longrightarrow> \<lparr>s;f;[$C (ConstInt32 k), $C v, $(Store t (Some tp) a off)]\<rparr> \<leadsto> \<lparr>s;f;[Trap]\<rparr>"
+| store_packed_Some:"\<lbrakk>(typeof_num v) = t; smem_ind (f_inst f) = Some j; ((mems s)!j) = m; store_packed m (nat_of_int k) off (bits_num v) (tp_num_length tp) = Some mem'\<rbrakk> \<Longrightarrow> \<lparr>s;f;[$C\<^sub>n (ConstInt32 k), $C\<^sub>n v, $(Store t (Some tp) a off)]\<rparr> \<leadsto> \<lparr>s\<lparr>mems:= ((mems s)[j := mem'])\<rparr>;f;[]\<rparr>"
+| store_packed_None:"\<lbrakk>(typeof_num v) = t; smem_ind (f_inst f) = Some j; ((mems s)!j) = m; store_packed m (nat_of_int k) off (bits_num v) (tp_num_length tp) = None\<rbrakk> \<Longrightarrow> \<lparr>s;f;[$C\<^sub>n (ConstInt32 k), $C\<^sub>n v, $(Store t (Some tp) a off)]\<rparr> \<leadsto> \<lparr>s;f;[Trap]\<rparr>"
+  \<comment> \<open>\<open>load vector\<close>\<close>
+| load_vec_Some:"\<lbrakk>smem_ind (f_inst f) = Some j; ((mems s)!j) = m; load_vec lv m (nat_of_int k) off = Some bs\<rbrakk> \<Longrightarrow> \<lparr>s;f;[$C\<^sub>n (ConstInt32 k), $(Load_vec lv a off)]\<rparr> \<leadsto> \<lparr>s;f;[$C\<^sub>v (ConstVec128 (deserialise_v128 bs))]\<rparr>"
+| load_vec_None:"\<lbrakk>smem_ind (f_inst f) = Some j; ((mems s)!j) = m; load_vec lv m (nat_of_int k) off = None\<rbrakk> \<Longrightarrow> \<lparr>s;f;[$C\<^sub>n (ConstInt32 k), $(Load_vec lv a off)]\<rparr> \<leadsto> \<lparr>s;f;[Trap]\<rparr>"
+  \<comment> \<open>\<open>load lane vector\<close>\<close>
+| load_lane_vec_Some:"\<lbrakk>smem_ind (f_inst f) = Some j; ((mems s)!j) = m; load m (nat_of_int k) off (vec_i_length svi) = Some bs\<rbrakk> \<Longrightarrow> \<lparr>s;f;[$C\<^sub>n (ConstInt32 k), $C\<^sub>v (ConstVec128 v), $(Load_lane_vec svi i a off)]\<rparr> \<leadsto> \<lparr>s;f;[$C\<^sub>v (ConstVec128 (insert_lane_vec svi i bs v))]\<rparr>"
+| load_lane_vec_None:"\<lbrakk>smem_ind (f_inst f) = Some j; ((mems s)!j) = m; load m (nat_of_int k) off (vec_i_length svi) = None\<rbrakk> \<Longrightarrow> \<lparr>s;f;[$C\<^sub>n (ConstInt32 k), $C\<^sub>v (ConstVec128 v), $(Load_lane_vec svi i a off)]\<rparr> \<leadsto> \<lparr>s;f;[Trap]\<rparr>"
+  \<comment> \<open>\<open>store vector\<close>\<close>
+| store_vec_Some:"\<lbrakk>smem_ind (f_inst f) = Some j; ((mems s)!j) = m; (store_serialise_vec sv v) = bs; store m (nat_of_int k) off bs (length bs) = Some mem'\<rbrakk> \<Longrightarrow> \<lparr>s;f;[$C\<^sub>n (ConstInt32 k), $C\<^sub>v (ConstVec128 v), $(Store_vec sv a off)]\<rparr> \<leadsto> \<lparr>s\<lparr>mems:= ((mems s)[j := mem'])\<rparr>;f;[]\<rparr>"
+| store_vec_None:"\<lbrakk>smem_ind (f_inst f) = Some j; ((mems s)!j) = m; (store_serialise_vec sv v) = bs; store m (nat_of_int k) off bs (length bs) = None\<rbrakk> \<Longrightarrow> \<lparr>s;f;[$C\<^sub>n (ConstInt32 k), $C\<^sub>v (ConstVec128 v), $(Store_vec sv a off)]\<rparr> \<leadsto> \<lparr>s;f;[Trap]\<rparr>"
   \<comment> \<open>\<open>current_memory\<close>\<close>
-| current_memory:"\<lbrakk>smem_ind (f_inst f) = Some j; ((mems s)!j) = m; mem_size m = n\<rbrakk> \<Longrightarrow> \<lparr>s;f;[ $(Current_memory)]\<rparr> \<leadsto> \<lparr>s;f;[$C (ConstInt32 (int_of_nat n))]\<rparr>"
+| current_memory:"\<lbrakk>smem_ind (f_inst f) = Some j; ((mems s)!j) = m; mem_size m = n\<rbrakk> \<Longrightarrow> \<lparr>s;f;[ $(Current_memory)]\<rparr> \<leadsto> \<lparr>s;f;[$C\<^sub>n (ConstInt32 (int_of_nat n))]\<rparr>"
   \<comment> \<open>\<open>grow_memory\<close>\<close>
-| grow_memory:"\<lbrakk>smem_ind (f_inst f) = Some j; ((mems s)!j) = m; mem_size m = n; mem_grow m (nat_of_int c) = Some mem'\<rbrakk> \<Longrightarrow> \<lparr>s;f;[$C (ConstInt32 c), $(Grow_memory)]\<rparr> \<leadsto> \<lparr>s\<lparr>mems:= ((mems s)[j := mem'])\<rparr>;f;[$C (ConstInt32 (int_of_nat n))]\<rparr>"
+| grow_memory:"\<lbrakk>smem_ind (f_inst f) = Some j; ((mems s)!j) = m; mem_size m = n; mem_grow m (nat_of_int c) = Some mem'\<rbrakk> \<Longrightarrow> \<lparr>s;f;[$C\<^sub>n (ConstInt32 c), $(Grow_memory)]\<rparr> \<leadsto> \<lparr>s\<lparr>mems:= ((mems s)[j := mem'])\<rparr>;f;[$C\<^sub>n (ConstInt32 (int_of_nat n))]\<rparr>"
   \<comment> \<open>\<open>grow_memory fail\<close>\<close>
-| grow_memory_fail:"\<lbrakk>smem_ind (f_inst f) = Some j; ((mems s)!j) = m; mem_size m = n\<rbrakk> \<Longrightarrow> \<lparr>s;f;[$C (ConstInt32 c),$(Grow_memory)]\<rparr> \<leadsto> \<lparr>s;f;[$C (ConstInt32 int32_minus_one)]\<rparr>"
-  (* The bad ones. *)
+| grow_memory_fail:"\<lbrakk>smem_ind (f_inst f) = Some j; ((mems s)!j) = m; mem_size m = n\<rbrakk> \<Longrightarrow> \<lparr>s;f;[$C\<^sub>n (ConstInt32 c),$(Grow_memory)]\<rparr> \<leadsto> \<lparr>s;f;[$C\<^sub>n (ConstInt32 int32_minus_one)]\<rparr>"
+  \<comment> \<open>\<open>block\<close>\<close>
+| block:"\<lbrakk>length vs = n; tb_tf (f_inst f) tb = (t1s _> t2s); length t1s = n; length t2s = m\<rbrakk> \<Longrightarrow> \<lparr>s;f;($C* vs) @ [$(Block tb es)]\<rparr> \<leadsto> \<lparr>s;f;[Label m [] (($C* vs) @ ($* es))]\<rparr>"
+  \<comment> \<open>\<open>loop\<close>\<close>
+| loop:"\<lbrakk>length vs = n; tb_tf (f_inst f) tb = (t1s _> t2s); length t1s = n; length t2s = m\<rbrakk> \<Longrightarrow> \<lparr>s;f;($C* vs) @ [$(Loop tb es)]\<rparr> \<leadsto> \<lparr>s;f;[Label n [$(Loop tb es)] (($C* vs) @ ($* es))]\<rparr>"
+  (* The bad ones *)
   \<comment> \<open>\<open>inductive label reduction\<close>\<close>
 | label:"\<lbrakk>\<lparr>s;f;es\<rparr> \<leadsto> \<lparr>s';f';es'\<rparr>; Lfilled k lholed es les; Lfilled k lholed es' les'\<rbrakk> \<Longrightarrow> \<lparr>s;f;les\<rparr> \<leadsto> \<lparr>s';f';les'\<rparr>"
   \<comment> \<open>\<open>inductive local reduction\<close>\<close>
 | local:"\<lbrakk>\<lparr>s;f;es\<rparr> \<leadsto> \<lparr>s';f';es'\<rparr>\<rbrakk> \<Longrightarrow> \<lparr>s;f0;[Frame n f es]\<rparr> \<leadsto> \<lparr>s';f0;[Frame n f' es']\<rparr>"
+  (* instantiation helpers *)
+| init_mem_Some:"\<lbrakk>smem_ind (f_inst f) = Some j; ((mems s)!j) = m; store m n 0 bs (length bs) = Some mem'\<rbrakk> \<Longrightarrow> \<lparr>s;f;[Init_mem n bs]\<rparr> \<leadsto> \<lparr>s\<lparr>mems:= ((mems s)[j := mem'])\<rparr>;f;[]\<rparr>"
+| init_mem_None:"\<lbrakk>smem_ind (f_inst f) = Some j; ((mems s)!j) = m; store m n 0 bs (length bs) = None\<rbrakk> \<Longrightarrow> \<lparr>s;f;[Init_mem n bs]\<rparr> \<leadsto> \<lparr>s;f;[Trap]\<rparr>"
+| init_tab_Some:"\<lbrakk>stab_ind (f_inst f) = Some j; ((tabs s)!j) = t; store_tab t n icls = Some tab'\<rbrakk> \<Longrightarrow> \<lparr>s;f;[Init_tab n icls]\<rparr> \<leadsto> \<lparr>s\<lparr>tabs:= ((tabs s)[j := tab'])\<rparr>;f;[]\<rparr>"
+| init_tab_None:"\<lbrakk>stab_ind (f_inst f) = Some j; ((tabs s)!j) = t; store_tab t n icls = None\<rbrakk> \<Longrightarrow> \<lparr>s;f;[Init_tab n icls]\<rparr> \<leadsto> \<lparr>s;f;[Trap]\<rparr>"
 
 definition reduce_trans where
   "reduce_trans \<equiv> (\<lambda>(s,f,es) (s',f',es'). \<lparr>s;f;es\<rparr> \<leadsto> \<lparr>s';f';es'\<rparr>)^**"
@@ -238,5 +288,19 @@ definition reduce_irrtrans where
 lemma reduce_irrtrans_trans:"reduce_irrtrans a b \<Longrightarrow> reduce_trans a b"
   unfolding reduce_irrtrans_def reduce_trans_def
   by simp
+
+type_synonym v_stack = "v list"
+
+abbreviation v_stack_to_es :: " v_stack \<Rightarrow> e list"
+  where "v_stack_to_es v \<equiv> $C* (rev v)"
+
+
+definition "computes cfg s' vs \<equiv> \<exists>f'. reduce_trans cfg (s', f', v_stack_to_es vs)"
+  
+definition "traps cfg s' \<equiv> \<exists>f'. reduce_trans cfg (s',f',[Trap])"
+
+definition "empty_frame \<equiv> \<lparr>f_locs = [],f_inst = \<lparr> types = [], funcs = [], tabs = [], mems = [], globs = []\<rparr>\<rparr>"
+
+definition "invoke_config s vargs i \<equiv> (s, empty_frame, ($C* vargs) @ [Invoke i])"
 
 end
