WebAssembly/Wasm_Countable.thy
@@ -1,0 +1,160 @@
+theory Wasm_Countable imports Wasm_Base_Defs "HOL-Library.Countable" begin
+
+instance t_num :: countable
+  by countable_datatype
+
+instance t_vec :: countable
+  by countable_datatype
+
+instance t :: countable
+  by countable_datatype
+
+instance tf :: countable
+  by countable_datatype
+
+instance tb :: countable
+  by countable_datatype
+
+instance inst_ext :: (countable) countable
+proof(rule countable_classI[of "\<lambda>i. to_nat (types i, inst.funcs i, inst.tabs i, inst.mems i, inst.globs i, inst.more i)"])
+qed auto
+
+instance tp_num :: countable
+  by countable_datatype
+
+instance tp_vec :: countable
+  by countable_datatype
+
+instance sx :: countable
+  by countable_datatype
+
+instance sat :: countable
+  by countable_datatype
+
+instance i32 :: countable
+proof(rule countable_classI[of "\<lambda>n::i32. nat_of_int n"])
+qed (simp add: Rep_i32_inject nat_of_int_i32.rep_eq)
+
+instance i64 :: countable
+proof(rule countable_classI[of "\<lambda>n::i64. nat_of_int n"])
+qed (simp add: Rep_i64_inject nat_of_int_i64.rep_eq)
+
+instance f32 :: countable
+proof(rule countable_classI[of "unat o Rep_f32"])
+qed (simp add: Rep_f32_inject)
+
+instance f64 :: countable
+proof(rule countable_classI[of "unat o Rep_f64"])
+qed (simp add: Rep_f64_inject)
+
+instance v128 :: countable
+proof(rule countable_classI[of "unat o Rep_v128"])
+qed (simp add: Rep_v128_inject)
+  
+instance v_num :: countable
+  by countable_datatype
+
+instance v_vec :: countable
+  by countable_datatype
+
+instance v :: countable
+  by countable_datatype
+
+instance unop_i :: countable
+  by countable_datatype
+
+instance unop_f :: countable
+  by countable_datatype
+
+instance unop :: countable
+  by countable_datatype
+
+instance binop_i :: countable
+  by countable_datatype
+
+instance binop_f :: countable
+  by countable_datatype
+
+instance binop :: countable
+  by countable_datatype
+
+instance testop :: countable
+  by countable_datatype
+
+instance relop_i :: countable
+  by countable_datatype
+
+instance relop_f :: countable
+  by countable_datatype
+
+instance relop :: countable
+  by countable_datatype
+
+instance cvtop :: countable
+  by countable_datatype
+
+instance shape_vec_i :: countable
+  by countable_datatype
+
+instance shape_vec_f :: countable
+  by countable_datatype
+
+instance shape_vec :: countable
+  by countable_datatype
+
+instance unop_vec :: countable ..
+
+instance binop_vec :: countable ..
+
+instance ternop_vec :: countable ..
+
+instance testop_vec :: countable ..
+
+instance shiftop_vec :: countable ..
+
+instance loadop_vec :: countable
+  by countable_datatype
+
+instance storeop_vec :: countable
+  by countable_datatype
+
+instance b_e :: countable
+  by countable_datatype
+
+axiomatization where
+  host_countable: "OFCLASS(host, countable_class)"
+
+instance host :: countable
+  by (rule host_countable)
+
+instance cl :: countable
+  by countable_datatype
+
+instance uint8 :: countable
+proof(rule countable_classI[of "\<lambda>n::byte. nat_of_byte n"])
+qed (simp add: Rep_uint8_inject nat_of_byte_def nat_of_uint8.rep_eq)
+
+instance mem_rep :: countable
+proof(rule countable_classI[of "\<lambda>m::mem_rep. to_nat (Rep_mem_rep m)"])
+qed (simp add: Rep_mem_rep_inject)
+
+instance mut :: countable
+  by countable_datatype
+
+instance global_ext :: (countable) countable
+proof(rule countable_classI[of "\<lambda>g. to_nat (g_mut g, g_val g, global.more g)"])
+qed simp
+
+instance s_ext :: (countable) countable
+proof (rule countable_classI[of "\<lambda>s. to_nat (funcs s, tabs s, mems s, globs s, s.more s)"])
+qed simp
+
+instance limit_t_ext :: (countable) countable
+proof (rule countable_classI[of "\<lambda>i. to_nat (l_min i, l_max i, limit_t.more i)"])
+qed simp
+
+instance tg_ext :: (countable) countable
+proof (rule countable_classI[of "\<lambda>i. to_nat (tg_mut i, tg_t i, tg.more i)"])
+qed simp
+
+end
